# baseURI: http://www.w3.org/ns/ssn-sosa
# imports: http://www.w3.org/ns/sosa/
# imports: http://www.w3.org/ns/ssn/
# prefix: ssn-sosa

@prefix dc: <http://purl.org/dc/elements/1.1/> .
@prefix dcterms: <http://purl.org/dc/terms/> .
@prefix owl: <http://www.w3.org/2002/07/owl#> .
@prefix rdf: <http://www.w3.org/1999/02/22-rdf-syntax-ns#> .
@prefix rdfs: <http://www.w3.org/2000/01/rdf-schema#> .
@prefix sosa: <http://www.w3.org/ns/sosa/> .
@prefix ssn: <http://www.w3.org/ns/ssn/> .
@prefix ssn-sosa: <http://www.w3.org/ns/ssn-sosa#> .
@prefix xsd: <http://www.w3.org/2001/XMLSchema#> .

sosa:ObservableProperty
  rdfs:comment "ssn:Property is super-class of all properties including those that are not necessarily 'observable'. " ;
  rdfs:subClassOf ssn:Property ;
.
sosa:hasValue
  rdfs:comment "Not clear how to relate this to ssn:hasValue, which is an owl:ObjectProperty" ;
.
<http://www.w3.org/ns/ssn-sosa>
  rdf:type owl:Ontology ;
  dc:contributor <https://www.w3.org/2000/09/dbwg/details?group=75471&public=1> ;
  dc:creator <http://orcid.org/0000-0002-3884-3420> ;
  dcterms:created "2017-01-24"^^xsd:date ;
  dcterms:modified "2017-02-08"^^xsd:date ;
  rdfs:comment "An initial mapping from SSN to SOSA" ;
  rdfs:seeAlso <https://www.w3.org/2015/spatial/wiki/Mapping_Table> ;
  owl:imports sosa: ;
  owl:imports ssn: ;
.
ssn:FeatureOfInterest
  owl:equivalentClass sosa:FeatureOfInterest ;
.
ssn:Observation
  owl:equivalentClass sosa:Observation ;
.
ssn:ObservationValue
  rdfs:subClassOf sosa:Result ;
.
ssn:Platform
  rdfs:comment "Unclear if ssn:Platform is as general as sosa:Platform since sosa:Platform explicitly mentions actuators and sampling devices." ;
  rdfs:subClassOf sosa:Platform ;
.
ssn:Process
  rdfs:comment "Relationship with sosa:Procedure unclear" ;
.
ssn:Property
  rdfs:comment "ssn:Property is super-class of some properties that are not necessarily 'observable'. Might be best as a super-property of sosa:ObservableProperty" ;
.
ssn:Sensor
  owl:equivalentClass sosa:Sensor ;
.
ssn:SensorOutput
  rdfs:subClassOf sosa:Result ;
.
ssn:attachedSystem
  owl:equivalentProperty sosa:hosts ;
.
ssn:featureOfInterest
  owl:equivalentProperty sosa:hasFeatureOfInterest ;
.
ssn:madeObservation
  owl:equivalentProperty sosa:madeObservation ;
.
ssn:observationResult
  rdfs:comment "sosa:hasResult also applies to actuation and sampling" ;
  rdfs:subPropertyOf sosa:hasResult ;
.
ssn:observationResultTime
  rdfs:comment "sosa:resultTime also applies to actuation and sampling" ;
  rdfs:subPropertyOf sosa:resultTime ;
.
ssn:observationSamplingTime
  rdfs:comment "Appears to be equivalent to sosa:phenomenonTime. Looks like SSN used a pre-standard version of O&M when selecting local-names." ;
  owl:equivalentProperty sosa:phenomenonTime ;
.
ssn:observedProperty
  owl:equivalentProperty sosa:observedProperty ;
.
ssn:observes
  owl:equivalentProperty sosa:observes ;
.
ssn:onPlatform
  owl:equivalentProperty sosa:hostedBy ;
.
ssn:sensingMethodUsed
  rdfs:comment "sosa:usedProcedure also applies to actuation and sampling" ;
  rdfs:subPropertyOf sosa:usedProcedure ;
.
